Proof of concept 128 bit load store

src/YulPrimops.ec
@@ -10,16 +10,128 @@ module Primops = {
   var memory : mem
   var reverted : bool
 
-  proc mload(a : uint256) : uint256 = {
-    return memory.[a];
+  proc mload(idx : uint256) : uint256 = {
+    (* _1 is the most significant byte *)
+    var _1, _2; (*, _3, _4, _5, _6, _7, _8, _9, _10, _11, _12, _13, _14, _15, _16, _17, _18, _19, _20, _21, _22, _23, _24, _25, _26, _27, _28, _29, _30, _31, _32; *)
+
+
+    _1 <- memory.[idx] `<<<` 128;
+    _2 <- memory.[idx+ W256.of_int 1] `<<<` 0;
+
+    
+
+
+    (* _3 <- memory.[idx+ W256.of_int 2] `<<<` 232;
+    _4 <- memory.[idx+ W256.of_int 3] `<<<` 224;
+    _5 <- memory.[idx+ W256.of_int 4] `<<<` 216;
+    _6 <- memory.[idx+ W256.of_int 5] `<<<` 208;
+    _7 <- memory.[idx+ W256.of_int 6] `<<<` 200;
+    _8 <- memory.[idx+ W256.of_int 7] `<<<` 192;
+    _9 <- memory.[idx+ W256.of_int 8] `<<<` 184;
+    _10 <- memory.[idx+ W256.of_int 9] `<<<` 176;
+    _11 <- memory.[idx+ W256.of_int 10] `<<<` 168;
+    _12 <- memory.[idx+ W256.of_int 11] `<<<` 160;
+    _13 <- memory.[idx+ W256.of_int 12] `<<<` 152;
+    _14 <- memory.[idx+ W256.of_int 13] `<<<` 144;
+    _15 <- memory.[idx+ W256.of_int 14] `<<<` 136;
+    _16 <- memory.[idx+ W256.of_int 15] `<<<` 128;
+    _17 <- memory.[idx+ W256.of_int 16] `<<<` 120;
+    _18 <- memory.[idx+ W256.of_int 17] `<<<` 112;
+    _19 <- memory.[idx+ W256.of_int 18] `<<<` 104;
+    _20 <- memory.[idx+ W256.of_int 19] `<<<` 96;
+    _21 <- memory.[idx+ W256.of_int 20] `<<<` 88;
+    _22 <- memory.[idx+ W256.of_int 21] `<<<` 80;
+    _23 <- memory.[idx+ W256.of_int 22] `<<<` 72;
+    _24 <- memory.[idx+ W256.of_int 23] `<<<` 64;
+    _25 <- memory.[idx+ W256.of_int 24] `<<<` 56;
+    _26 <- memory.[idx+ W256.of_int 25] `<<<` 48;
+    _27 <- memory.[idx+ W256.of_int 26] `<<<` 40;
+    _28 <- memory.[idx+ W256.of_int 27] `<<<` 32;
+    _29 <- memory.[idx+ W256.of_int 28] `<<<` 24;
+    _30 <- memory.[idx+ W256.of_int 29] `<<<` 16;
+    _31 <- memory.[idx+ W256.of_int 30] `<<<` 8;
+    _32 <- memory.[idx+ W256.of_int 31]; *)
+    return (
+      _1 +
+      _2 (* +
+      _3 +
+      _4 +
+      _5 +
+      _6 +
+      _7 +
+      _8 +
+      _9 +
+      _10 +
+      _11 +
+      _12 +
+      _13 +
+      _14 +
+      _15 +
+      _16 +
+      _17 +
+      _18 +
+      _19 +
+      _20 +
+      _21 +
+      _22 +
+      _23 +
+      _24 +
+      _25 +
+      _26 +
+      _27 +
+      _28 +
+      _29 +
+      _30 +
+      _31 +
+      _32 *)
+    );
   }
 
-  proc mstore(a : uint256, v : uint256): unit = {
-    memory <- memory.[a<-v];
+  proc mstore(idx : uint256, val : uint256): unit = {
+    var _1, _2;
+    (* memory <- memory.[(idx + W256.of_int 31)<-(val `&` W256.masklsb 8)];
+    memory <- memory.[(idx + W256.of_int 30)<-((val `>>>` 8) `&` W256.masklsb 8)];
+    memory <- memory.[(idx + W256.of_int 29)<-((val `>>>` 16) `&` W256.masklsb 8)];
+    memory <- memory.[(idx + W256.of_int 28)<-((val `>>>` 24) `&` W256.masklsb 8)];
+    memory <- memory.[(idx + W256.of_int 27)<-((val `>>>` 32) `&` W256.masklsb 8)];
+    memory <- memory.[(idx + W256.of_int 26)<-((val `>>>` 40) `&` W256.masklsb 8)];
+    memory <- memory.[(idx + W256.of_int 25)<-((val `>>>` 48) `&` W256.masklsb 8)];
+    memory <- memory.[(idx + W256.of_int 24)<-((val `>>>` 56) `&` W256.masklsb 8)];
+    memory <- memory.[(idx + W256.of_int 23)<-((val `>>>` 64) `&` W256.masklsb 8)];
+    memory <- memory.[(idx + W256.of_int 22)<-((val `>>>` 72) `&` W256.masklsb 8)];
+    memory <- memory.[(idx + W256.of_int 21)<-((val `>>>` 80) `&` W256.masklsb 8)];
+    memory <- memory.[(idx + W256.of_int 20)<-((val `>>>` 88) `&` W256.masklsb 8)];
+    memory <- memory.[(idx + W256.of_int 19)<-((val `>>>` 96) `&` W256.masklsb 8)];
+    memory <- memory.[(idx + W256.of_int 18)<-((val `>>>` 104) `&` W256.masklsb 8)];
+    memory <- memory.[(idx + W256.of_int 17)<-((val `>>>` 112) `&` W256.masklsb 8)];
+    memory <- memory.[(idx + W256.of_int 16)<-((val `>>>` 120) `&` W256.masklsb 8)];
+    memory <- memory.[(idx + W256.of_int 15)<-((val `>>>` 128) `&` W256.masklsb 8)];
+    memory <- memory.[(idx + W256.of_int 14)<-((val `>>>` 136) `&` W256.masklsb 8)];
+    memory <- memory.[(idx + W256.of_int 13)<-((val `>>>` 144) `&` W256.masklsb 8)];
+    memory <- memory.[(idx + W256.of_int 12)<-((val `>>>` 152) `&` W256.masklsb 8)];
+    memory <- memory.[(idx + W256.of_int 11)<-((val `>>>` 160) `&` W256.masklsb 8)];
+    memory <- memory.[(idx + W256.of_int 10)<-((val `>>>` 168) `&` W256.masklsb 8)];
+    memory <- memory.[(idx + W256.of_int 9)<-((val `>>>` 176) `&` W256.masklsb 8)];
+    memory <- memory.[(idx + W256.of_int 8)<-((val `>>>` 184) `&` W256.masklsb 8)];
+    memory <- memory.[(idx + W256.of_int 7)<-((val `>>>` 192) `&` W256.masklsb 8)];
+    memory <- memory.[(idx + W256.of_int 6)<-((val `>>>` 200) `&` W256.masklsb 8)];
+    memory <- memory.[(idx + W256.of_int 5)<-((val `>>>` 208) `&` W256.masklsb 8)];
+    memory <- memory.[(idx + W256.of_int 4)<-((val `>>>` 216) `&` W256.masklsb 8)];
+    memory <- memory.[(idx + W256.of_int 3)<-((val `>>>` 224) `&` W256.masklsb 8)];
+    memory <- memory.[(idx + W256.of_int 2)<-((val `>>>` 232) `&` W256.masklsb 8)]; *)
+
+    (* memory <- memory.[(idx + W256.of_int 1)<-((val `>>>` 0) `&` W256.masklsb 128)];
+    memory <- memory.[idx<-((val `>>>` 128) `&` W256.masklsb 128)]; *)
+
+    _1 <- (splitMask (W256.masklsb 128) val).`2 `>>>` 128;
+    _2 <- (splitMask (W256.masklsb 128) val).`1;
+
+    memory <- memory.[idx<-_1];
+    memory <- memory.[(idx+W256.of_int 1)<-_2];
   }
 
-  proc mstore8(a : uint256, v : uint256) : unit = {
-    (* TODO: memory model? *)
+  proc mstore8(idx : uint256, val : uint256) : unit = {
+    memory <- memory.[idx<-(val `&` W256.masklsb 8)];
   }
 
   proc ret(retOff : uint256, retSize : uint256) : unit = {
