src/zksync_verifier.ec
@@ -6,7 +6,7 @@ op p = W256.of_int 2188824287183927522224640574525727508869631115729782366268903
 
 module Test = {
 
-  proc pointNegate(point : uint256) : unit = {
+    proc pointNegate(point : uint256) : unit = {
       var _1, _2, _3, pY, tmp166, tmp167, tmp168, _6, _7;
       _1 <- W256.of_int 32;
       _2 <- point + _1;
@@ -28,6 +28,12 @@ module Test = {
       }
     }
 
+        proc writeReadTest(address: uint256, value: uint256): uint256 = {
+      var _1;
+        Primops.mstore(address, value);
+        _1 <@ Primops.mload(address);
+        return _1;
+    }
 }.
 
 (* Some potentially useful lemmas to prove mid-level specs *)
@@ -45,11 +51,60 @@ lemma mod_mod_eq_mod :
     forall (m1 m2 v : int), 0 < m1 => m1 <= m2 => (v %% m1) %% m2 = v %% m1.
     progress.
     smt ().
+  qed.
+
+lemma add_one_neq:
+    forall (x: uint256), x <> x + W256.one.
+    proof.
+      progress.
+      smt.
     qed.
 
+lemma shl_zero:
+    forall (x: uint256), x `<<<` 0 = x.
+    progress.
+    apply W256.ext_eq.
+    progress.
+    smt.
+  qed.
+
+lemma splitmask2_shr_shl:
+    forall (x: uint256) (i: int),
+    (0 <= i /\ i < 256) => (splitMask (W256.masklsb i) x).`2 `>>>` i `<<<` i = (splitMask (W256.masklsb i) x).`2.
+    proof.
+      progress.
+      apply W256.ext_eq.
+      progress.
+      rewrite /splitMask.
+      simplify.
+      smt.
+    qed.
+  
 (* Functional correctness *)
 
-
+  lemma writeReadTest_correctness :
+      forall (address value: uint256),
+  hoare [ Test.writeReadTest :
+        arg = (address, value) ==>
+        res = value].
+      proof.
+        progress.
+        proc.
+        inline Primops.mstore Primops.mload.
+        wp.
+        skip.
+        progress.
+        rewrite Map.get_set_sameE Map.get_set_neqE.
+        apply add_one_neq.
+        rewrite Map.get_set_sameE.
+        rewrite shl_zero.
+        rewrite splitmask2_shr_shl.
+        trivial.
+        rewrite addrC.
+        rewrite splitMask_add.
+      reflexivity.
+qed.
+      
 lemma pointNegate_correctness :
     forall (x y point_addr : uint256),
 hoare [ Test.pointNegate :
